proof of link with simple decisiveOp & flow.v restructuring

flows.v
@@ -9,13 +9,13 @@ From iris.algebra Require Export auth agree.
 
 (* ---------- Flow Interface encoding and camera definitions ---------- *)
 
-(* This section is proved in Grasshopper *)
+(* This section is proved in the appendix *)
 
 Definition key := nat.
 
 Definition node := nat.
 
-Parameter flowdom: Set.
+Definition flowdom := nat.
 
 Record flowintT :=
   {
@@ -23,7 +23,7 @@ Record flowintT :=
     out : gmap node flowdom;
     dom : gset node;
   }.
-
+  
 Canonical Structure flowintRAC := leibnizO flowintT.
 
 Instance flowintRAop : Op flowintT.
@@ -38,7 +38,7 @@ Proof. Admitted.
 Instance flowintRAunit : cmra.Unit flowintT.
 Proof. Admitted.
 
-Definition flowintRA_mixin : RAMixin flowintT.
+Definition flowintRA_mixin : RAMixin flowintT.        (* separate proofs and admits of flowint RA *) 
 Proof.
   split; try apply _; try done.
 Admitted.
@@ -53,67 +53,24 @@ Proof. Admitted.
 
 Lemma flowint_ucmra_mixin : UcmraMixin flowintT.
 Proof. Admitted.
+
 Canonical Structure flowintUR : ucmraT := UcmraT flowintT flowint_ucmra_mixin.
 
-Parameter in_inset : key → flowintUR → node → Prop.
-Parameter in_edgeset : key → flowintUR → node → node → Prop.
-Parameter in_outset : key → flowintUR → node → Prop.
-Parameter not_in_outset : key → flowintUR → node → Prop.
-Parameter cont : node → gset key.
-Parameter inreach : flowintUR → node → gset key.
-Parameter intLeq : flowintUR → flowintUR → Prop.
-Parameter is_empty_flowint : flowintUR → Prop.
-Parameter globalint : flowintUR → Prop.           (* Need to discuss *)
-
-(* ---------- Lemmas about flow interfaces proved in the appendix : ---------- *)
-
-(* Directly follows from definition of composition *)
-Lemma flowint_comp_fp (I1 I2 I : flowintUR) : I = I1 ⋅ I2 → dom I = dom I1 ∪ dom I2.
-Proof. Admitted.
+Parameter contextualLeq : flowintUR → flowintUR → Prop.
 
 (* Directly follows from definition of contextual extension *)
-Lemma intLeq_impl_fp I I' : intLeq I I' → dom I ⊆ dom I'.
+Lemma contextualLeq_impl_fp I I' : contextualLeq I I' → dom I = dom I'.
 Proof. Admitted.
 
 (* This is the rule AUTH-FI-UPD in the paper *)
 Definition flowint_update_P (I I_n I_n': flowintUR) (x : authR flowintUR) : Prop :=
   match (auth_auth_proj x) with
   | Some (q, z) => ∃ I', (z = to_agree(I')) ∧ q = 1%Qp ∧ (I_n' = auth_frag_proj x) 
-                        ∧ intLeq I I' ∧ ∃ I_o, I = I_n ⋅ I_o ∧ I' = I_n' ⋅ I_o
+                        ∧ contextualLeq I I' ∧ ∃ I_o, I = I_n ⋅ I_o ∧ I' = I_n' ⋅ I_o
   | _ => False
   end.
 
-
 Lemma flowint_update I I_n I_n' :
-  intLeq I_n I_n' → (● I ⋅ ◯ I_n) ~~>: (flowint_update_P I I_n I_n').
-Proof. Admitted.
-
-(* ---------- Proved in GRASShopper for each implementation: ---------- *)
-
-Lemma inreach_impl_inset I_n n k:
-  dom I_n = {[n]} → k ∈ inreach I_n n ∧ not_in_outset k I_n n ∧ ✓ I_n → in_inset k I_n n.
-Proof. Admitted.
-
-Lemma flowint_inset_step I1 n I2 n' k :
-  dom I1 = {[n]} → dom I2 = {[n']} → ✓(I1 ⋅ I2)
-  → in_inset k I1 n → in_edgeset k I1 n n' → in_inset k I2 n'.        (* in_edgeset interpretation? *)
-Proof. Admitted.
-
-Lemma flowint_inreach_step (I I1 I2: flowintUR) k n n':
-  dom I1 = {[n]} → n' ∈ dom I2 → I = I1 ⋅ I2 → ✓(I)
-  → k ∈ inreach I n → in_edgeset k I1 n n' → k ∈ inreach I n'.
-Proof. Admitted.
-
-Lemma flowint_proj I I_n n k :
-  I_n ≼ I → ✓I → in_inset k I n → in_inset k I_n n.
-Proof. Admitted.
-
-Lemma flowint_step (I I1 I2: flowintUR) k n n':
-  I = I1 ⋅ I2 → ✓I → n ∈ dom I1 → in_edgeset k I1 n n' → globalint I → n' ∈ dom I2.
-Proof. Admitted.
-
-(** Proved in multiset-flows.spl *)
-Lemma flowint_step_gh (I I1 I2: flowintUR) k n:
-  I = I1 ⋅ I2 → ✓I → in_outset k I1 n → globalint I → n ∈ dom I2.
+  contextualLeq I_n I_n' → (● I ⋅ ◯ I_n) ~~>: (flowint_update_P I I_n I_n').
 Proof. Admitted.
 
