link.v
@@ -91,33 +91,55 @@ Section Link_Template.
   Notation iProp := (iProp Σ).
 
   (* ---------- Flow interface set-up specific to this proof ---------- *)
+  
+  Parameter in_inset : key → flowintUR → node → Prop.
+  Parameter in_outset : key → flowintUR → node → Prop.
+  Parameter not_in_outset : key → flowintUR → Prop.
+  Parameter inreach : flowintUR → node → gset key.
+  Parameter is_empty_flowint : flowintUR → Prop.
 
   Variable root : node.    (* make root parameter of the specs *)
-  Variable KS : gset key.
+  Variable KS : gset key.                                
   Variable hrep : node → flowintUR → gset key → iProp.
   Parameter hrep_timeless_proof : ∀ n I C, Timeless (hrep n I C).
   Instance hrep_timeless n I C: Timeless (hrep n I C).
   Proof. apply hrep_timeless_proof. Qed.
-  Parameter hrep_fp : ∀ n I_n C, hrep n I_n C -∗ ⌜Nds I_n = {[n]}⌝.
   Parameter hrep_sep_star: ∀ n I_n I_n' C C', hrep n I_n C ∗ hrep n I_n' C' -∗ False.
   Parameter KS_full : ∀ k, k ∈ KS.
-  
-  Hypothesis globalint_root_fp: ∀ I, globalint I → root ∈ Nds I.
 
-  Hypothesis contextualLeq_impl_globalint :
-    ∀ I I', globalint I →  contextualLeq I I' → globalint I'.
+  Definition globalint I : Prop := ✓I ∧ (∀ k n, ¬ (in_outset k I n)) ∧  (* For later, make outset and inset to be sets *)
+                                  (∀ n, (n = root) → (∀ k, in_inset k I n ∧ k ∈ inreach I n)
+                                      ∧ (n ≠ root) → (∀ k, ¬ in_inset k I n ∧ k ∉ inreach I n)).  
 
-  Hypothesis keyset_in_out : ∀ k In n, in_inset k In n → not_in_outset k In n → k ∈ ks n.
+  (* ---------- Proved in GRASShopper for each implementation: ---------- *)
+
+  Lemma flowint_comp_fp (I1 I2 I : flowintUR) : I = I1 ⋅ I2 → dom I = dom I1 ∪ dom I2.
+  Proof. Admitted.
+
+  Hypothesis globalint_root_fp: ∀ I, globalint I → root ∈ dom I.
+
+  Hypothesis keyset_in_out : ∀ k In n, in_inset k In n → not_in_outset k In → k ∈ ks n.
   
-  Hypothesis globalint_root_inr : ∀ I k, globalint I → k ∈ inreach I root.
+  Hypothesis globalint_root_inr : ∀ I k, globalint I → k ∈ inreach I root. (* can be proved in coq itself *)
 
   Hypothesis globalint_inreach :
-    ∀ I1 I n, I1 ≼ I → Nds I1 = {[n]} → globalint I → inreach I1 n = inreach I n.
+    ∀ Ir I, Ir ≼ I → dom Ir = {[root]} → globalint I → inreach Ir root = inreach I root.
+      
+  Hypothesis outset_distinct : ∀ I n, (∃ k, in_outset k I n) → n ∉ dom I. 
+  
+  Lemma inreach_impl_inset I_n n k:
+    dom I_n = {[n]} → k ∈ inreach I_n n ∧ not_in_outset k I_n ∧ ✓ I_n → in_inset k I_n n.
+  Proof. Admitted.
 
-  Hypothesis globalint_preserve_inreach : ∀ I I' I_n I_n' n,
-      ✓ I → ✓ I' → (∃ I_o, I = I_n ⋅ I_o ∧ I' = I_n' ⋅ I_o) → globalint I
-      → Nds I_n = {[n]} → Nds I_n' = {[n]} → inreach I_n n = inreach I_n' n
-      → ∀ n', n' ∈ Nds I' → inreach I n' = inreach I' n'.
+  Lemma flowint_inreach_step (I I1 I2: flowintUR) k n n':
+    dom I1 = {[n]} → n' ∈ dom I2 → I = I1 ⋅ I2 → ✓(I)
+    → k ∈ inreach I1 n → in_outset k I1 n' → k ∈ inreach I2 n'.
+  Proof. Admitted.
+
+  Lemma flowint_step (I I1 I2: flowintUR) k n:
+    I = I1 ⋅ I2 → ✓I → in_outset k I1 n → globalint I → n ∈ dom I2.
+  Proof. Admitted.
+
 
   (* ---------- Coarse-grained specification ---------- *)
 
@@ -144,30 +166,28 @@ Section Link_Template.
            findNext #n #k
        {{{ (b: bool) (n': node), 
               RET (match b with true => (SOMEV #n') | false => NONEV end); 
-               hrep n I_n C ∗ (match b with true => ⌜in_edgeset k I_n n n'⌝ |
-                                          false => ⌜not_in_outset k I_n n⌝ end) }}})%I.
+               hrep n I_n C ∗ (match b with true => ⌜in_outset k I_n n'⌝ |
+                                          false => ⌜not_in_outset k I_n⌝ end) }}})%I.
 
-(* deal with contextualLeq *)
   Parameter decisiveOp_spec : ∀ (dop: dOp) (n: node) (k: key) (I_n: flowintUR) (C: gset key),
       ({{{ hrep n I_n C ∗ ⌜in_inset k I_n n⌝
-                    ∗ ⌜not_in_outset k I_n n⌝ }}}
+                    ∗ ⌜not_in_outset k I_n⌝ }}}
            decisiveOp dop #n #k
-       {{{ (b: bool) (I_n': flowintUR) (C': gset key) (res: bool),
+       {{{ (b: bool) (C': gset key) (res: bool),
                   RET (match b with false => NONEV | true => (SOMEV #res) end);
                   match b with false => hrep n I_n C |
-                              true => hrep n I_n' C' ∗ Ψ dop k C C' res ∗ ⌜ C' ⊆ ks n⌝
-                                      ∗ ⌜contextualLeq I_n I_n'⌝ ∗ ⌜Nds I_n' = {[n]}⌝ 
-                                      ∗ ⌜inreach I_n n = inreach I_n' n⌝  end }}})%I.
+                              true => hrep n I_n C' ∗ Ψ dop k C C' res ∗ ⌜ C' ⊆ ks n⌝ end }}})%I.
 
   (* ---------- The invariant ---------- *)
-
-  Definition searchStr γ γ_fp γ_k γ_inr γ_fi I C : iProp :=
-    (own γ (● I) ∗ own γ_k (● prod (KS, C)) ∗ own γ_fp (● Nds I) ∗ ⌜globalint I⌝
-      ∗ ([∗ set] n ∈ (Nds I), (∃ (b: bool) (In: flowintUR),
+  
+(* should change the name so as to not confuse with the node-level predicate *)
+  Definition searchStr γ γ_fp γ_k γ_inr γ_fi I C : iProp :=                             
+    (own γ (● I) ∗ own γ_k (● prod (KS, C)) ∗ own γ_fp (● dom I) ∗ ⌜globalint I⌝
+      ∗ ([∗ set] n ∈ (dom I), (∃ (b: bool) (In: flowintUR),
           (lockLoc n) ↦ #b
           ∗ (if b then True
             else (∃ Cn, hrep n In Cn ∗ own (γ_fi n) ((●{1/2} In)) ∗ own γ_k (◯ prod (ks(n), Cn))))
-          ∗ own γ (◯ In) ∗ ⌜Nds In = {[n]}⌝ ∗ own (γ_fi n) ((●{1/2} In)) ∗ own (γ_inr n) (● (inreach In n))
+          ∗ own γ (◯ In) ∗ ⌜dom In = {[n]}⌝ ∗ own (γ_fi n) ((●{1/2} In)) ∗ own (γ_inr n) (● (inreach In n))
         ))
     )%I.    
 
@@ -221,8 +241,6 @@ Section Link_Template.
               ✓ prod (KS, C) ∧ ✓ prod (K1, Cn) ∧ k ∈ K1 ∧ k ∉ Cn →
              (prod (KS, C), prod (K1, Cn)) ~l~> (prod (KS, C ∪ {[k]}), prod (K1, Cn ∪ {[k]})).
   Proof.
-  Admitted.
-(*  
     intros [H1 [H2 [H3 H4]]]. apply local_update_discrete. intros z.
     intros _. intros. split. rewrite /(✓ prod (KS, C ∪ {[k]})) /=. 
     rewrite /(cmra_valid keysetRA) /=. rewrite /(✓ prod (KS, C)) /= in H1.
@@ -242,13 +260,11 @@ Section Link_Template.
     rewrite /(op) /=. rewrite /(cmra_op keysetRA) /=. done.
     rewrite /(opM) /=. inversion H. done.
   Qed.
-*)
+
   Lemma auth_ks_local_update_delete K1 C Cn k:
               ✓ prod (KS, C) ∧ ✓ prod (K1, Cn) ∧ k ∈ K1 ∧ k ∈ Cn →
              (prod (KS, C), prod (K1, Cn)) ~l~> (prod (KS, C ∖ {[k]}), prod (K1, Cn ∖ {[k]})).
   Proof.
-  Admitted.
-(*
     intros [H1 [H2 [H3 H4]]]. apply local_update_discrete. intros z.
     intros _. intros. split. rewrite /(✓ prod (KS, C ∖ {[k]})) /=. 
     rewrite /(cmra_valid keysetRA) /=. rewrite /(✓ prod (KS, C)) /= in H1.
@@ -269,95 +285,8 @@ Section Link_Template.
     rewrite /(op) /=. rewrite /(cmra_op keysetRA) /=. done.
     rewrite /(opM) /=. inversion H. done.
   Qed.
-*)
-         
-  Lemma flowint_update_result γ I I_n I_n' x :
-    ⌜flowint_update_P I I_n I_n' x⌝ ∧ own γ x -∗
-                       ∃ I', ⌜contextualLeq I I'⌝ ∗ ⌜∃ I_o, I = I_n ⋅ I_o ∧ I' = I_n' ⋅ I_o⌝
-                                ∗ own γ (● I' ⋅ ◯ I_n').
-  Proof.
-    unfold flowint_update_P.
-    case_eq (auth_auth_proj x); last first.
-    - intros H. iIntros "(% & ?)". iExFalso. done.
-    - intros p. intros H. case_eq p. intros q a Hp.
-      iIntros "[% Hown]". destruct H0 as [I' H0].
-      destruct H0. destruct H1. destruct H2. destruct H3.
-      iExists I'.
-      iSplit. iPureIntro. apply H3.
-      iSplit. iPureIntro. apply H4.
-      assert (Auth (auth_auth_proj x) (auth_frag_proj x) = x) as Hx.
-      { destruct x. reflexivity. }
-      assert (x = (Auth (Some (1%Qp, to_agree(I'))) (I_n'))) as H'.
-      { rewrite <-Hx. rewrite H. rewrite <-H2. rewrite Hp. rewrite H1.
-       rewrite H0. reflexivity. }
-      assert (● I' = Auth (Some (1%Qp, to_agree(I'))) ε) as HI'. { reflexivity. }
-      assert (◯ I_n' = Auth ε I_n') as HIn'. { reflexivity. }
-      assert (ε ⋅ I_n' = I_n') as HeIn.
-      { rewrite /(⋅) /=. rewrite left_id. done. }
-      assert (Some (1%Qp, to_agree I') ⋅ None = Some (1%Qp, to_agree I')) as Hs.
-      { rewrite /(⋅) /=.
-        rewrite /(cmra_op (optionR (prodR fracR (agreeR flowintUR))) (Some (1%Qp, to_agree I')) (None)) /=.
-        reflexivity. }
-      assert (● I' ⋅ ◯ I_n' = (Auth (Some (1%Qp, to_agree(I'))) (I_n'))) as Hd.
-      { rewrite /(● I') /= /(◯ I_n') /=. rewrite /(⋅) /=.
-        rewrite /(cmra_op (authR flowintUR) (Auth (Some (1%Qp, to_agree I')) ε) (Auth None I_n')) /=.
-        rewrite /auth_op /=. rewrite HeIn. rewrite Hs. reflexivity. }
-      iEval (rewrite Hd). iEval (rewrite <- H'). done.
-  Qed.
 
-  Lemma inv_impl_fp γ γ_fp γ_k γ_inr γ_fi n I Ns C:
-    searchStr γ γ_fp γ_k γ_inr γ_fi I C ∗ own γ_fp (◯ Ns) ∗ ⌜n ∈ Ns⌝ -∗ ⌜n ∈ Nds I⌝.
-  Proof. Admitted.
 
-(*    iIntros "(HInv & HNs & %)".
-    iDestruct "HInv" as "(? & HIns & ? & ? & HNs' & %)".
-    iPoseProof (auth_set_incl with "[$HNs $HNs']") as "%".
-    iPureIntro. set_solver.
-  Qed.                                       (* Made Proof using Type* *)
-*)
-
-  Lemma inv_impl_inreach γ γ_fp γ_k γ_inr γ_fi n I C Inr :
-    searchStr γ γ_fp γ_k γ_inr γ_fi I C ∗ own (γ_inr n) (◯ Inr) ∗ ⌜n ∈ Nds I⌝
-    -∗ ⌜Inr ⊆ inreach I n⌝.
-  Proof. Admitted.
-
-(*    iIntros "(HInv & HInr & %)".
-    iDestruct "HInv" as "(? & ? & ? & ? & HIns & HNs' & % & HInrs)".
-    iPoseProof ((big_sepS_elem_of_acc _ (Nds I) n) with "[$HInrs]") as "(HInr' & HInrRest)";
-      first done.
-    iDestruct "HInr'" as (Inr') "(HInr' & %)".
-    rewrite <- H1.
-    iApply (auth_set_incl with "[$HInr $HInr']").
-  Qed.
-*)
-
-  Lemma inv_impl_inreach_eq γ γ_fp γ_k γ_inr γ_fi I C n I_n C_n :
-    searchStr γ γ_fp γ_k γ_inr γ_fi I C ∗ own γ (◯ I_n) ∗ hrep n I_n C_n
-    -∗ ⌜inreach I n = inreach I_n n⌝.
-  Proof. Admitted.
-
-(*    iIntros "(HInv & HIn & Hg)".
-    iDestruct "HInv" as "(? & ? & HI & % & HIns & HNs' & % & HInrs)".
-    iPoseProof (auth_own_incl γ I I_n with "[$HI $HIn]") as "%".
-    iPoseProof (hrep_fp n I_n with "Hg") as "%".
-    iPureIntro.
-    by rewrite (globalint_inreach I_n I).
-  Qed.
-*)
-
-(*  Lemma rewrite_inside_big_sep I I' γ_inr :
-    ([∗ set] n ∈ Nds I', (∃ Inr_n : gsetUR key,
-                            own (γ_inr n) (● Inr_n) ∗ ⌜Inr_n = inreach I n⌝))
-      -∗ ⌜∀ n', n' ∈ Nds I' → inreach I n' = inreach I' n'⌝
-      -∗ ([∗ set] n ∈ Nds I', (∃ Inr_n : gsetUR key,
-                                 own (γ_inr n) (● Inr_n) ∗ ⌜Inr_n = inreach I' n⌝)).
-  Proof.
-    iIntros "Hbig %" .
-    iApply (big_sepS_mono _ _ (Nds I') with "Hbig").
-    intros. iIntros "H".
-    specialize a with x. apply a in H. rewrite H. done.
-  Qed.
-*)
   (* ---------- Lock module proofs ---------- *)
 
   Lemma lockNode_spec (n: node):
@@ -399,179 +328,13 @@ Section Link_Template.
   Qed.
 
   (* ---------- Ghost state manipulation to make final proof cleaner ---------- *)
-(*
-  Lemma ghost_update_step γ γ_fp γ_inr γ_c (n n': node) (k:key) (Ns: gset node) (I_n: flowintUR) (Inr: gset key):
-          is_dict γ γ_fp γ_inr γ_c -∗ own γ_fp (◯ Ns) ∗ ⌜n ∈ Ns⌝∗ own (γ_inr n) (◯ Inr) ∗ ⌜k ∈ Inr⌝ ∗ own γ (◯ I_n)
-                                      ∗ ⌜Nds I_n = {[n]}⌝ ∗ ⌜in_edgeset k I_n n n'⌝
-                    ={ ⊤ }=∗ ∃ Ns' Inr', own γ_fp (◯ Ns') ∗ ⌜n' ∈ Ns'⌝ ∗ own (γ_inr n') (◯ Inr') ∗ ⌜k ∈ Inr'⌝
-                                        ∗ own γ (◯ I_n).
-  Proof.
-    iIntros "#HInv (#Hfp & #Hin & #Hinr & #Hkin & HIn & #HNds & #Hedge)".
-    iInv dictN as ">H". iDestruct "H" as (I Ns' C) "H". 
-    iPoseProof (inv_impl_fp n Ns with "[$H $Hfp $Hin]") as "%".
-    iPoseProof (inv_impl_inreach with "[$H $Hinr //]") as "%".
-    iDestruct "H" as "(HC & #HCI & HI & #Hglob & Hstar & HAuthfp & #HINds & Hbinr)".
-    iPoseProof (auth_own_incl with "[$HI $HIn]") as "%".
-    unfold included in H1. destruct H1 as [I2 Hmult].
-    iPoseProof ((own_valid γ (● I)) with "HI") as "%".
-    iDestruct "HNds" as %HNds. iDestruct "Hglob" as %Hglob.
-    iDestruct "Hedge" as %Hedge. iDestruct "Hkin" as %Hkin.
-    assert (n' ∈ Nds I2).
-    { apply (flowint_step I I_n _ k n). done. apply auth_auth_valid; try done.
-      replace (Nds I_n). set_solver. done. done. }
-    iAssert (⌜n' ∈ Nds I⌝)%I as "%".
-    { iPureIntro.
-      apply flowint_comp_fp in Hmult. set_solver.
-    }
-    iMod (own_update γ_fp (● Ns') (● Ns' ⋅ ◯ Ns') with "HAuthfp") as "HNs".
-    apply auth_update_core_id. apply gset_core_id. done.
-    iEval (rewrite own_op) in "HNs". iDestruct "HNs" as "(HNs0 & HNs')".
-    iPoseProof ((big_sepS_elem_of_acc _ (Nds I) n') with "[$Hbinr]") as "(HInrn' & HInrRest)";
-      first done.
-    iDestruct "HInrn'" as (Inr') "[HInr' %]".
-    iMod (own_update (γ_inr n') (● Inr') (● Inr' ⋅ ◯ Inr') with "HInr'") as "HInr'".
-    apply auth_update_core_id. apply gset_core_id. done.
-    iEval (rewrite own_op) in "HInr'". iDestruct "HInr'" as "(HInr0 & HInr')".
-    iPoseProof ("HInrRest" with "[HInr0]") as "HInrs".
-    { iExists (Inr'). by iFrame. }
-    iAssert (⌜k ∈ Inr'⌝)%I as "%".
-    { replace Inr'. iPureIntro.
-      apply (flowint_inreach_step I I_n I2 _ n); try done.
-        apply auth_auth_valid. done. try set_solver.
-    }
-    iModIntro. iSplitR "HNs' HInr' HIn". iNext. iExists I, Ns', C.
-    iFrame "HC HI Hstar HNs0 HInrs". try repeat iSplitL; done.
-    iModIntro. iExists Ns', Inr'. iFrame "HNs' HInr' HIn".
-    iDestruct "HINds" as %HINds. iPureIntro. set_solver. 
-  Qed.
-
-  Lemma ghost_update_traverse γ γ_fp γ_inr γ_c (k:key):
-          is_dict γ γ_fp γ_inr γ_c -∗ True ={ ⊤ }=∗ ∃ Ns Inr, own γ_fp (◯ Ns) ∗ ⌜root ∈ Ns⌝ 
-                                                              ∗ own (γ_inr root) (◯ Inr) ∗ ⌜k ∈ Inr⌝.
-  Proof.  
-    iIntros "#HInv #Ht". iInv dictN as ">H".
-    iDestruct "H" as (I Ns C) "(HC & % & HI & % & HIns & HNs & % & HInrs)".
-    iMod (own_update γ_fp (● Ns) (● Ns ⋅ ◯ Ns) with "HNs") as "HNs".
-    apply auth_update_core_id. apply gset_core_id. done.
-    iEval (rewrite own_op) in "HNs". iDestruct "HNs" as "(HNs & #HNs')".
-    iAssert (⌜root ∈ Nds I⌝ ∗ ⌜k ∈ inreach I root⌝)%I as "[% %]".
-    { iPureIntro. split. by apply globalint_root_fp. by apply globalint_root_inr. }
-    iPoseProof ((big_sepS_elem_of_acc _ (Nds I) root) with "[$HInrs]") as "(HInrRoot & HInrRest)";
-    first done. iDestruct "HInrRoot" as (Inr) "[HInr %]".
-    iMod (own_update (γ_inr root) (● Inr) (● Inr ⋅ ◯ Inr) with "HInr") as "HInr".
-    apply auth_update_core_id. apply gset_core_id. done.
-    iEval (rewrite own_op) in "HInr". iDestruct "HInr" as "(HInr0 & HInr)".
-    iPoseProof ("HInrRest" with "[HInr0]") as "HInrs".
-    { iExists (Inr). by iFrame. }
-    iAssert (⌜k ∈ Inr⌝)%I as "%". by replace Inr.
-    iModIntro. iSplitR "HNs' HInr". iNext. iExists I, Ns, C. iFrame "# % ∗".
-    iModIntro. iExists Ns, Inr. iFrame "HInr HNs'". iPureIntro. set_solver. 
-  Qed.
-
-  Lemma ghost_update_decisiveOp γ γ_fp γ_inr γ_c (n: node) (k:key) (Ns: gset node) (I_n: flowintUR) (Inr: gset key):
-          is_dict γ γ_fp γ_inr γ_c -∗ own γ_fp (◯ Ns) ∗ ⌜n ∈ Ns⌝ ∗ own (γ_inr n) (◯ Inr) ∗ ⌜k ∈ Inr⌝
-                                        ∗ own γ (◯ I_n) ∗ hrep n I_n ∗ ⌜not_in_outset k I_n n⌝
-                    ={ ⊤ }=∗ ⌜in_inset k I_n n⌝ ∗ hrep n I_n ∗ own γ (◯ I_n).
-  Proof.
-    iIntros "#Hinv  (HNs & % & HInr & % & HIn & Hg & %)".
-    iInv dictN as ">HInv" "HClose".
-    iDestruct "HInv" as (I Ns' C) "HInv".
-    iPoseProof (inv_impl_fp n Ns with "[$HInv $HNs //]") as "%".
-    (* k ∈ Inr → k ∈ inreach I n *)
-    iPoseProof (inv_impl_inreach with "[$HInv $HInr //]") as "%".
-    iPoseProof (inv_impl_inreach_eq n with "[$HInv $HIn $Hg //]") as "%".
-    iPoseProof (auth_frag_valid γ with "HIn") as "%".
-    iMod ("HClose" with "[-HInr Hg HIn]").
-    { iNext. iExists I, Ns', C. done. }
-    iPoseProof (hrep_fp n I_n with "Hg") as "%".
-    iModIntro. iFrame. iPureIntro.
-    apply inreach_impl_inset; try done. repeat split; try done.
-    set_solver.
-  Qed.
-*)
-  (* ---------- Refinement proofs ---------- *)
-
-  Lemma traverse_spec (γ γ_fp γ_k: gname) γ_inr γ_fi (k: key) (n: node) (Ns: gset node) (I_n:flowintUR) :
-       ⌜n ∈ Ns⌝ ∗ own γ_fp (◯ Ns) ∗ ⌜root ∈ Ns⌝ ∗ own (γ_inr n) (◯ (inreach I_n n)) ∗ ⌜k ∈ inreach I_n n⌝ -∗ 
-          <<< ∀ C, is_searchStr γ γ_fp γ_k γ_inr γ_fi C >>>
-                traverse #n #k
-                    @ ⊤
-          <<< ∃ (n': node) (Ns': gsetUR node) (I_n': flowintUR) (Cn': gset key),
-                           is_searchStr γ γ_fp γ_k γ_inr γ_fi C ∗ ⌜n' ∈ Ns'⌝ ∗ own γ_fp (◯ Ns') ∗  hrep n' I_n' Cn' 
-                         ∗ own (γ_fi n') ((●{1/2} I_n')) ∗ own γ_k (◯ prod (ks(n'), Cn'))
-                         ∗ ⌜in_inset k I_n' n'⌝ ∗ ⌜not_in_outset k I_n' n'⌝, RET #n' >>>.
-  Proof.
-    iLöb as "IH" forall (n Ns I_n). iIntros "(#Hinn & #Hfp & #Hroot & #Hinrfp & #Hkinr)".
-    iDestruct "Hinn" as %Hinn. iDestruct "Hroot" as %Hroot.
-    iIntros (Φ) "AU". wp_lam. wp_let. wp_bind(lockNode _)%E.
-    awp_apply (lockNode_spec n). iApply (aacc_aupd_abort with "AU"); first done.
-    iIntros (C0) "Hst". iDestruct "Hst" as (I) "(HI & HKS & HNDS & Hglob & Hstar)".
-    iAssert (⌜n ∈ Nds I⌝)%I with "[HNDS]" as "%".
-    { iPoseProof ((auth_set_incl γ_fp Ns (Nds I)) with "[$]") as "%".
-      iPureIntro. set_solver. }
-    rewrite (big_sepS_elem_of_acc _ (Nds I) n); last by eauto.
-    iDestruct "Hstar" as "[Hn Hstar]".
-    iDestruct "Hn" as (b In) "(Hlock & Hb & HIn & #HNds & Hfis & Hks)".
-    iAaccIntro with "Hlock". { iIntros "H". iModIntro. iSplitL. iFrame "∗ % #".
-    iExists I. iFrame "∗ % #". iApply "Hstar". iExists b, In.
-    iFrame "# % ∗". eauto with iFrame. } iIntros "(Hloc & ?)".
-    destruct b. { iExFalso. done. } iModIntro. 
-    iPoseProof (auth_set_incl with "[$Hks $Hinrfp]") as "%".
-    iDestruct "Hkinr" as "%". assert (k ∈ inreach In n) as Hkinr. { set_solver. } 
-    iSplitR "Hb". iFrame "∗ % #". iExists I. iFrame "∗ % #". iApply "Hstar". iExists true, In.
-    iFrame "# % ∗". iIntros "AU". iModIntro. wp_pures.
-    iDestruct "Hb" as (Cn) "(Hrep & Hfil & Hks)". iDestruct "HNds" as %HNds.
-    wp_bind (findNext _ _)%E. wp_apply ((findNext_spec n In Cn k) with "[Hrep]").
-    iFrame; iPureIntro; done. iIntros (b n') "(Hrep & Hb)". destruct b. 
-    - wp_pures. awp_apply (unlockNode_spec n). 
-      iApply (aacc_aupd_abort with "AU"); first done. iIntros (C1) "Hst".
-      iDestruct "Hst" as (I1) "(HI & HKS & HNDS & Hglob & Hstar)".
-      iAssert (⌜n ∈ Nds I1⌝)%I with "[HNDS]" as "%".
-      { iPoseProof ((auth_set_incl γ_fp Ns (Nds I1)) with "[$]") as "%".
-        iPureIntro. set_solver. }
-      rewrite (big_sepS_delete _ (Nds I1) n); last by eauto. iDestruct "Hstar" as "(Hcln & Hstar)".
-      iDestruct "Hcln" as (b In1) "(Hlock & Hbb & HIn & #HNds1 & Hfis & Hks1)".
-      destruct b; first last. { iDestruct "Hbb" as (Cn') "(Hrep' & _)".
-      iAssert (⌜False⌝)%I with "[Hrep Hrep']" as %Hf. { iApply (hrep_sep_star n In In1). 
-      iFrame. } exfalso. done. }
-      iPoseProof ((own_valid_2 (γ_fi n) (●{1 / 2} In) (●{1 / 2} In1)) with "[Hfil] [Hfis]") as "%"; try done.
-      apply (auth_auth_frac_op_inv _ _ _ _) in H3. apply leibniz_equiv in H3. replace In1.            
-      iDestruct "Hb" as %Hb. iDestruct "HNds1" as %HNds1. iDestruct "Hglob" as %Hglob.
-      iPoseProof (auth_own_incl with "[$HI $HIn]") as (I2)"%".
-      iPoseProof (own_valid with "HI") as "%". iAssert (⌜n' ∈ Nds I1⌝)%I as "%".
-      { iPureIntro. assert (n' ∈ Nds I2). { apply (flowint_step I1 In _ k n). done. 
-        apply auth_auth_valid. done. replace (Nds In). set_solver. done. done. }
-        apply flowint_comp_fp in H4. set_solver. }
-      rewrite (big_sepS_delete _ (Nds I1 ∖ {[n]}) n'); last first. admit. iDestruct "Hstar" as "(Hcln' & Hstar)".
-      iDestruct "Hcln'" as (b In') "(Hlock' & Hbb' & HIn' & #HNds' & Hfis' & Hks1')".
-      assert (k ∈ inreach In' n'). { admit. } assert (root ∈ Nds I1). { apply globalint_root_fp. done. }
-      iMod (own_update (γ_inr n') (● inreach In' n') (● inreach In' n' ⋅ ◯ inreach In' n') with "Hks1'") as "HNs".
-      apply auth_update_core_id. apply gset_core_id. done. iDestruct "HNs" as "(Hks1' & #Hinr1')".
-      iAaccIntro with "Hlock". { iIntros "Hlock". iModIntro. iSplitR "Hfil Hks Hrep". iFrame "∗ # %".
-      iExists I1. iFrame "∗ % #". rewrite (big_sepS_delete _ (Nds I1) n); last by eauto.
-      iSplitR "Hstar Hbb' HIn' Hfis' Hks1' Hlock'". iExists true, In. iFrame "# % ∗". 
-      rewrite (big_sepS_delete _ (Nds I1 ∖ {[n]}) n'); last first. admit. iFrame. iExists b, In'.
-      iFrame "# % ∗".  iIntros "AU". iModIntro. iFrame "# % ∗". } iIntros "Hlock".
-      iMod (own_update γ_fp (● Nds I1) (● Nds I1 ⋅ ◯ Nds I1) with "HNDS") as "HNs".
-      apply auth_update_core_id. apply gset_core_id. done. iDestruct "HNs" as "(HAfp & #Hfp1)".
-      iModIntro. iSplitL. iExists I1. iFrame "∗ % #". rewrite (big_sepS_delete _ (Nds I1) n); last by eauto.
-      iSplitR "Hstar Hbb' HIn' Hfis' Hks1' Hlock'". iExists false, In. iFrame "# % ∗". iExists Cn. iFrame. 
-      rewrite (big_sepS_delete _ (Nds I1 ∖ {[n]}) n'); last first. admit. iFrame. iExists b, In'.
-      iFrame "# % ∗". iIntros "AU". iModIntro. wp_pures. iSpecialize ("IH" $! n' (Nds I1) In').
-      iApply "IH". iFrame "∗ # %". done.
-    - iApply fupd_wp. iMod "AU" as (C) "[Hst [_ Hclose]]". iSpecialize ("Hclose" $! n Ns In Cn).
-      iMod ("Hclose" with "[Hst Hfil Hks Hrep Hb]") as "HΦ". iFrame "∗ # %". admit.
-      iModIntro. wp_pures. done.
-  Admitted.
-
-  (* ---------- Ghost state manipulation to make final proof cleaner ---------- *)
 
   Lemma ghost_update_keyset γ_k dop k Cn Cn' res K1 C:
           Ψ dop k Cn Cn' res ∗ own γ_k (● prod (KS, C)) ∗ own γ_k (◯ prod (K1, Cn))
                              ∗ ⌜Cn' ⊆ K1⌝ ∗ ⌜k ∈ K1⌝  ==∗
                  ∃ C', Ψ dop k C C' res ∗ own γ_k (● prod (KS, C')) ∗ own γ_k (◯ prod (K1, Cn')).
-  Proof. Admitted.
-(*    iIntros "(#HΨ & Ha & Hf & % & %)". iPoseProof (auth_own_incl_ks γ_k (prod (KS, C)) (prod (K1, Cn))
+  Proof.
+    iIntros "(#HΨ & Ha & Hf & % & %)". iPoseProof (auth_own_incl_ks γ_k (prod (KS, C)) (prod (K1, Cn))
                 with "[$Ha $Hf]") as "%".
     iPoseProof ((own_valid γ_k (● prod (KS, C))) with "Ha") as "%".
     iPoseProof ((own_valid γ_k (◯ prod (K1, Cn))) with "Hf") as "%".
@@ -620,7 +383,95 @@ Section Link_Template.
         * assert (Cn' = Cn). { set_solver. } iModIntro. iExists C. iEval (rewrite <-H13) in "Hf".
           iFrame. unfold Ψ. iPureIntro. set_solver.
   Qed.
-*)
+
+
+  (* ---------- Proofs of traverse and searchStrOp ---------- *)
+
+  Lemma traverse_spec (γ γ_fp γ_k: gname) γ_inr γ_fi (k: key) (n: node) (Ns: gset node) (I_n:flowintUR) :
+       ⌜n ∈ Ns⌝ ∗ own γ_fp (◯ Ns) ∗ ⌜root ∈ Ns⌝ ∗ own (γ_inr n) (◯ (inreach I_n n)) ∗ ⌜k ∈ inreach I_n n⌝ -∗ 
+          <<< ∀ C, is_searchStr γ γ_fp γ_k γ_inr γ_fi C >>>
+                traverse #n #k
+                    @ ⊤
+          <<< ∃ (n': node) (Ns': gsetUR node) (I_n': flowintUR) (Cn': gset key),
+                           is_searchStr γ γ_fp γ_k γ_inr γ_fi C ∗ ⌜n' ∈ Ns'⌝ ∗ own γ_fp (◯ Ns') ∗  hrep n' I_n' Cn' 
+                         ∗ own (γ_fi n') ((●{1/2} I_n')) ∗ own γ_k (◯ prod (ks(n'), Cn')) ∗ ⌜dom I_n' = {[n']}⌝
+                         ∗ ⌜in_inset k I_n' n'⌝ ∗ ⌜not_in_outset k I_n'⌝, RET #n' >>>.
+  Proof.
+    iLöb as "IH" forall (n Ns I_n). iIntros "(#Hinn & #Hfp & #Hroot & #Hinrfp & #Hkinr)".
+    iDestruct "Hinn" as %Hinn. iDestruct "Hroot" as %Hroot.
+    iIntros (Φ) "AU". wp_lam. wp_let. wp_bind(lockNode _)%E.
+    awp_apply (lockNode_spec n). iApply (aacc_aupd_abort with "AU"); first done.
+    iIntros (C0) "Hst". iDestruct "Hst" as (I) "(HI & HKS & HNDS & Hglob & Hstar)".
+    iAssert (⌜n ∈ dom I⌝)%I with "[HNDS]" as "%".
+    { iPoseProof ((auth_set_incl γ_fp Ns (dom I)) with "[$]") as "%".
+      iPureIntro. set_solver. }
+    rewrite (big_sepS_elem_of_acc _ (dom I) n); last by eauto.
+    iDestruct "Hstar" as "[Hn Hstar]".
+    iDestruct "Hn" as (b In) "(Hlock & Hb & HIn & #HNds & Hfis & Hks)".
+    iAaccIntro with "Hlock". { iIntros "H". iModIntro. iSplitL. iFrame "∗ % #".
+    iExists I. iFrame "∗ % #". iApply "Hstar". iExists b, In.
+    iFrame "# % ∗". eauto with iFrame. } iIntros "(Hloc & ?)".
+    destruct b. { iExFalso. done. } iModIntro. 
+    iPoseProof (auth_set_incl with "[$Hks $Hinrfp]") as "%".
+    iDestruct "Hkinr" as "%". assert (k ∈ inreach In n) as Hkinr. { set_solver. }
+    iPoseProof (own_valid with "HIn") as "%". rename H2 into HInV.
+    assert (✓ In) as HInv. { apply (auth_frag_valid (◯ In)). done. }
+    iSplitR "Hb". iFrame "∗ % #". iExists I. iFrame "∗ % #". iApply "Hstar". iExists true, In.
+    iFrame "# % ∗". iIntros "AU". iModIntro. wp_pures.
+    iDestruct "Hb" as (Cn) "(Hrep & Hfil & Hks)". iDestruct "HNds" as %HNds.
+    wp_bind (findNext _ _)%E. wp_apply ((findNext_spec n In Cn k) with "[Hrep]").
+    iFrame; iPureIntro; done. iIntros (b n') "(Hrep & Hb)". destruct b. 
+    - wp_pures. awp_apply (unlockNode_spec n). 
+      iApply (aacc_aupd_abort with "AU"); first done. iIntros (C1) "Hst".
+      iDestruct "Hst" as (I1) "(HI & HKS & HNDS & Hglob & Hstar)".
+      iAssert (⌜n ∈ dom I1⌝)%I with "[HNDS]" as "%".
+      { iPoseProof ((auth_set_incl γ_fp Ns (dom I1)) with "[$]") as "%".
+        iPureIntro. set_solver. }
+      rewrite (big_sepS_delete _ (dom I1) n); last by eauto. iDestruct "Hstar" as "(Hcln & Hstar)".
+      iDestruct "Hcln" as (b In1) "(Hlock & Hbb & HIn & #HNds1 & Hfis & Hks1)".
+      destruct b; first last. { iDestruct "Hbb" as (Cn') "(Hrep' & _)".
+      iAssert (⌜False⌝)%I with "[Hrep Hrep']" as %Hf. { iApply (hrep_sep_star n In In1). 
+      iFrame. } exfalso. done. }
+      iPoseProof ((own_valid_2 (γ_fi n) (●{1 / 2} In) (●{1 / 2} In1)) with "[Hfil] [Hfis]") as "%"; try done.
+      apply (auth_auth_frac_op_inv _ _ _ _) in H3. apply leibniz_equiv in H3. replace In1.            
+      iDestruct "Hb" as %Hb. iDestruct "HNds1" as %HNds1. iDestruct "Hglob" as %Hglob.
+      iPoseProof (auth_own_incl with "[$HI $HIn]") as (I2)"%".
+      iPoseProof (own_valid with "HI") as "%". iAssert (⌜n' ∈ dom I1⌝)%I as "%".
+      { iPureIntro. assert (n' ∈ dom I2). { apply (flowint_step I1 In I2 k n'). done. 
+        apply auth_auth_valid. done. done. done. }
+        apply flowint_comp_fp in H4. set_solver. }
+      assert (n ≠ n') as Hneq. { assert (n' ∉ dom In). { apply (outset_distinct In n').
+      exists k. done. } rewrite HNds1 in H7. set_solver. }
+      rewrite (big_sepS_delete _ (dom I1 ∖ {[n]}) n'); last first.
+      set_solver. iDestruct "Hstar" as "(Hcln' & Hstar)". 
+      iDestruct "Hcln'" as (b In') "(Hlock' & Hbb' & HIn' & #HNds' & Hfis' & Hks1')".
+      iPoseProof ((own_op γ (◯ In) (◯ In' )) with "[HIn HIn']") as "H"; first by eauto with iFrame.
+      iPoseProof (own_valid with "H") as "%". rewrite -auth_frag_op in H7.
+      assert (✓ (In ⋅ In')). { apply (auth_frag_valid (◯ (In ⋅ In'))). done. }
+      iDestruct "HNds'" as %HNds'. assert (k ∈ inreach In' n').
+      { apply (flowint_inreach_step (In⋅In') In In' k n n'); try done. set_solver. }
+      assert (root ∈ dom I1). { apply globalint_root_fp. done. } iDestruct "H" as "(HIn & HIn')".
+      iMod (own_update (γ_inr n') (● inreach In' n') (● inreach In' n' ⋅ ◯ inreach In' n') with "Hks1'") as "HNs".
+      apply auth_update_core_id. apply gset_core_id. done. iDestruct "HNs" as "(Hks1' & #Hinr1')".
+      iAaccIntro with "Hlock". { iIntros "Hlock". iModIntro. iSplitR "Hfil Hks Hrep". iFrame "∗ # %".
+      iExists I1. iFrame "∗ % #". rewrite (big_sepS_delete _ (dom I1) n); last by eauto.
+      iSplitR "Hstar Hbb' HIn' Hfis' Hks1' Hlock'". iExists true, In. iFrame "# % ∗". 
+      rewrite (big_sepS_delete _ (dom I1 ∖ {[n]}) n'); last first. set_solver. iFrame. iExists b, In'.
+      iFrame "# % ∗".  iIntros "AU". iModIntro. iFrame "# % ∗". } iIntros "Hlock".
+      iMod (own_update γ_fp (● dom I1) (● dom I1 ⋅ ◯ dom I1) with "HNDS") as "HNs".
+      apply auth_update_core_id. apply gset_core_id. done. iDestruct "HNs" as "(HAfp & #Hfp1)".
+      iModIntro. iSplitL. iExists I1. iFrame "∗ % #". rewrite (big_sepS_delete _ (dom I1) n); last by eauto.
+      iSplitR "Hstar Hbb' HIn' Hfis' Hks1' Hlock'". iExists false, In. iFrame "# % ∗". iExists Cn. iFrame. 
+      rewrite (big_sepS_delete _ (dom I1 ∖ {[n]}) n'); last first. set_solver. iFrame. iExists b, In'.
+      iFrame "# % ∗". iIntros "AU". iModIntro. wp_pures. iSpecialize ("IH" $! n' (dom I1) In').
+      iApply "IH". iFrame "∗ # %". done.
+    - iApply fupd_wp. iMod "AU" as (C) "[Hst [_ Hclose]]". iSpecialize ("Hclose" $! n Ns In Cn).
+      iMod ("Hclose" with "[Hst Hfil Hks Hrep Hb]") as "HΦ". iDestruct "Hb" as %Hnotout.
+      iFrame "∗ # %". iPureIntro. apply (inreach_impl_inset In n k); try split; try done.
+      iModIntro. wp_pures. done.
+  Qed.
+
+
 
   Theorem searchStrOp_spec (γ γ_fp γ_k: gname) γ_inr γ_fi (k: key) (dop: dOp):
       <<< ∀ C, is_searchStr γ γ_fp γ_k γ_inr γ_fi C >>>
@@ -633,96 +484,80 @@ Section Link_Template.
     iApply fupd_wp. iMod "AU" as (C0) "[Hst [HAU _]]".
     iDestruct "Hst" as (I0) "(HI & HKS & HNDS & #Hglob & Hstar)".
     iDestruct "Hglob" as %Hglob. 
-    assert (root ∈ Nds I0)%I as Hroot. { apply globalint_root_fp. done. }
-    iMod (own_update γ_fp (● Nds I0) (● Nds I0 ⋅ ◯ Nds I0) with "HNDS") as "H".
+    assert (root ∈ dom I0)%I as Hroot. { apply globalint_root_fp. done. }
+    iMod (own_update γ_fp (● dom I0) (● dom I0 ⋅ ◯ dom I0) with "HNDS") as "H".
     { apply auth_update_core_id. apply gset_core_id. done. } 
     iDestruct "H" as "(HNDS & #Hfp0)".
-    rewrite (big_sepS_elem_of_acc _ (Nds I0) root); last by eauto.
+    rewrite (big_sepS_elem_of_acc _ (dom I0) root); last by eauto.
     iDestruct "Hstar" as "[Hn Hstar]".
     iDestruct "Hn" as (b Ir) "(H1 & H2 & H3 & H4 & H5 & Hksr)".
+    iPoseProof (auth_own_incl with "[$HI $H3]") as "%". iDestruct "H4" as %HNdsr.
+    assert (inreach Ir root = inreach I0 root) as Hinreach. { apply globalint_inreach; try done. }
     iMod (own_update (γ_inr root) (● inreach Ir root) (● inreach Ir root ⋅ ◯ inreach Ir root) with "Hksr") as "H".
     apply auth_update_core_id. apply gset_core_id. done. iDestruct "H" as "(Hksr & #Hinr)".
-    iMod ("HAU" with "[HI HKS H1 H2 H3 H4 H5 Hstar HNDS Hksr] ") as "AU". 
+    iMod ("HAU" with "[HI HKS H1 H2 H3 H5 Hstar HNDS Hksr] ") as "AU". 
     { iExists I0. iFrame "∗ % #". iApply "Hstar". iExists b, Ir. iFrame "∗ # %". }
     iModIntro. wp_bind (traverse _ _)%E.
-    awp_apply (traverse_spec γ γ_fp γ_k γ_inr γ_fi k root (Nds I0) Ir). iFrame "∗ # %". admit.
+    awp_apply (traverse_spec γ γ_fp γ_k γ_inr γ_fi k root (dom I0) Ir). iFrame "∗ # %".
+    iPureIntro. rewrite Hinreach. apply globalint_root_inr. done.
     iApply (aacc_aupd_abort with "AU"); first done.
     iIntros (C1) "Hst". iAaccIntro with "Hst"; first by eauto with iFrame.
-    iIntros (n Ns In Cn) "(Hst & #Hinn & #Hfp & Hrepn & Hfil & Hks & #Hinset & #Hnotout)".
+    iIntros (n Ns In Cn) "(Hst & #Hinn & #Hfp & Hrepn & Hfil & Hks & #HNdsn & #Hinset & #Hnotout)".
     iDestruct "Hinn" as %Hinn. iDestruct "Hinset" as %Hinset. iDestruct "Hnotout" as %Hnotout.
     iModIntro. iFrame. iIntros "AU". iModIntro. wp_pures. wp_bind (decisiveOp _ _ _)%E.
     wp_apply ((decisiveOp_spec dop n k In Cn) with "[Hrepn]"). eauto with iFrame.
-    iIntros (b' In' Cn' res). iIntros "Hb". destruct b'.
-    - iDestruct "Hb" as "(Hrep & #HΨ & #Hsub & #Hcon & #HNds' & #Hinreq)".
+    iIntros (b' Cn' res). iIntros "Hb". destruct b'.
+    - iDestruct "Hb" as "(Hrep & #HΨ & #Hsub)".
       wp_pures. wp_bind(unlockNode _)%E.
       awp_apply (unlockNode_spec n).
       iApply (aacc_aupd_commit with "AU"); first done. iIntros (C2) "Hst".
       iDestruct "Hst" as (I) "(HI & HKS & HNDS & #Hglob & Hstar)". 
       iDestruct "Hglob" as %Hglob'.
-      iAssert (⌜n ∈ Nds I⌝)%I with "[HNDS]" as "%".
-      { iPoseProof ((auth_set_incl γ_fp Ns (Nds I)) with "[$]") as "%".
+      iAssert (⌜n ∈ dom I⌝)%I with "[HNDS]" as "%".
+      { iPoseProof ((auth_set_incl γ_fp Ns (dom I)) with "[$]") as "%".
       iPureIntro. set_solver. }
-      rewrite (big_sepS_elem_of_acc _ (Nds I) n); last by eauto.
+      rewrite (big_sepS_elem_of_acc _ (dom I) n); last by eauto.
       iDestruct "Hstar" as "[Hn Hstar]".
       iDestruct "Hn" as (b' In1) "(Hlock & Hb & HIn & #HNds & Hfis & Hinreach)".
       destruct b'; first last. { iDestruct "Hb" as (Cn'') "(Hrep' & _)".
-      iAssert (⌜False⌝)%I with "[Hrep Hrep']" as %Hf. { iApply (hrep_sep_star n In' In1). 
+      iAssert (⌜False⌝)%I with "[Hrep Hrep']" as %Hf. { iApply (hrep_sep_star n In In1). 
       iFrame. } exfalso. done. }
       iAaccIntro with "Hlock". { iIntros "Hlock". iModIntro. iSplitR "Hfil Hrep Hks".
       iExists I. iFrame "∗ % #". iApply "Hstar". iExists true, In1. 
       iFrame "∗ # %". eauto with iFrame. } iIntros "Hlock".
       iPoseProof (auth_own_incl with "[$HI $HIn]") as (I2)"%".
-      iPoseProof ((own_valid γ (● I)) with "HI") as "%". iDestruct "Hcon" as %Hcon.
+      iPoseProof ((own_valid γ (● I)) with "HI") as "%".
       iPoseProof ((own_valid_2 (γ_fi n) (●{1 / 2} In) (●{1 / 2} In1)) with "[Hfil] [Hfis]") as "%"; try done.
-      apply (auth_auth_frac_op_inv _ _ _ _) in H2. apply leibniz_equiv in H2. replace In1.            
-      iMod (own_updateP (flowint_update_P I In In') γ (● I ⋅ ◯ In) with "[HI HIn]") as (?) "H0".
-      { apply (flowint_update I In In'). done. } { rewrite own_op. iFrame. }
-      iPoseProof ((flowint_update_result γ I In In') with "H0") as (I') "(% & % & HIIn)".
-      iAssert (own γ (● I') ∗ own γ (◯ In'))%I 
-                                with "[HIIn]" as "(HI' & HIn')". { by rewrite own_op. }
-      iPoseProof ((own_valid γ (● I')) with "HI'") as "%". iDestruct "Hsub" as "%".
+      apply (auth_auth_frac_op_inv _ _ _ _) in H3. apply leibniz_equiv in H3. replace In1.            
       iMod ((ghost_update_keyset γ_k dop k Cn Cn' res (ks n) C2) with "[HKS Hks]") as "Hgks".
       iFrame "% ∗ #". iPureIntro. apply (keyset_in_out k In n); try done. 
       iDestruct "Hgks" as (C2') "(#HΨC & Ha & Hf)".
-      iAssert (own (γ_fi n) (●{1/2} In ⋅ ●{1/2} In))%I with "[Hfil Hfis]" as "H".
-      { rewrite own_op. iFrame. } assert (∀ Iv: flowintUR, ●{1 / 2} Iv ⋅ ●{1 / 2} Iv ≡ ●{1/2 + 1/2} Iv) as Hv. 
-      { intros Iv. rewrite (auth_auth_frac_op ((1/2)%Qp) ((1/2)%Qp) Iv). done. } 
-      assert ((1/2 + 1/2)%Qp = (1)%Qp) as Hadd. { apply (Qp_div_2 1). }
-      rewrite Hadd in Hv. iEval (rewrite Hv) in "H". 
-      iPoseProof ((own_update (γ_fi n) (●In) (●In')) with "H") as ">Hγir".
-      { apply (auth_update_auth In In' ε). apply local_update_discrete. intros mz.
-        intros. admit. (* use contextualLeq *) } 
       iModIntro. iExists (C2'), res. iSplitL. iSplitR "HΨC".
-      { iExists I'. assert (globalint I') as HI'.
-      { apply (contextualLeq_impl_globalint I I'). done. done. }
-      assert (Nds I = Nds I') as HH. { apply (contextualLeq_impl_fp I I'). done. }
-      iEval (rewrite HH) in "Hstar". iEval (rewrite HH) in "HNDS". iFrame "∗ % #".
-      iApply "Hstar". iExists false, In'. iEval (rewrite <-Hv) in "Hγir".
-      iEval (rewrite own_op) in "Hγir". iDestruct "Hγir" as "(Hfil & Hfis)".
-      iDestruct "Hinreq" as %Hinreq. iEval (rewrite Hinreq) in "Hinreach". 
+      { iExists I. iFrame "∗ % #".
+      iApply "Hstar". iExists false, In. 
       iFrame "∗ % #". iExists Cn'. eauto with iFrame. } done.
       iIntros "HΦ". iModIntro. wp_pures. done.
     - wp_match. awp_apply (unlockNode_spec n).
       iApply (aacc_aupd_abort with "AU"); first done. iIntros (C2) "Hst".
       iDestruct "Hst" as (I) "(HI & HKS & HNDS & #Hglob & Hstar)". 
       iDestruct "Hglob" as %Hglob'.
-      iAssert (⌜n ∈ Nds I⌝)%I with "[HNDS]" as "%".
-      { iPoseProof ((auth_set_incl γ_fp Ns (Nds I)) with "[$]") as "%".
+      iAssert (⌜n ∈ dom I⌝)%I with "[HNDS]" as "%".
+      { iPoseProof ((auth_set_incl γ_fp Ns (dom I)) with "[$]") as "%".
       iPureIntro. set_solver. }
-      rewrite (big_sepS_elem_of_acc _ (Nds I) n); last by eauto.
+      rewrite (big_sepS_elem_of_acc _ (dom I) n); last by eauto.
       iDestruct "Hstar" as "[Hn Hstar]".
       iDestruct "Hn" as (b' In1) "(Hlock & Hb' & HIn & #HNds & Hfis & Hinreach)".
       destruct b'; first last. { iDestruct "Hb'" as (Cn'') "(Hrep' & _)".
-      iAssert (⌜False⌝)%I with "[Hb Hrep']" as %Hf. { iApply (hrep_sep_star n In' In1). 
-      iFrame. } exfalso. done. }
+      iAssert (⌜False⌝)%I with "[Hb Hrep']" as %Hf. { iApply (hrep_sep_star n In In1). 
+      iFrame "∗ # %". } exfalso. done. }
       iAaccIntro with "Hlock". { iIntros "Hlock". iModIntro. iSplitR "Hfil Hb Hks".
       iExists I. iFrame "∗ % #". iApply "Hstar". iExists true, In1. 
       iFrame "∗ # %". eauto with iFrame. } iIntros "Hlock". iModIntro.
       iPoseProof ((own_valid_2 (γ_fi n) (●{1 / 2} In) (●{1 / 2} In1)) with "[Hfil] [Hfis]") as "%"; try done.
-      apply (auth_auth_frac_op_inv _ _ _ _) in H0. apply leibniz_equiv in H0. replace In1.            
+      apply (auth_auth_frac_op_inv _ _ _ _) in H1. apply leibniz_equiv in H1. replace In1.            
       iSplitR "". iExists I. iFrame "∗ % #". iApply "Hstar". iExists false, In. iFrame "∗ % #".
       iExists Cn. iFrame. iIntros "AU". iModIntro. wp_pures. iApply "IH". done.
-  Admitted.
+  Qed.
  
 
 
